src/typechecker/FStarC.TypeChecker.Primops.Array.fst
@@ -1,5 +1,4 @@
 module FStarC.TypeChecker.Primops.Array
-#push-options "--MLish --MLish_effect FStarC.Effect"
 
 open FStarC
 open FStarC.Effect
@@ -18,25 +17,25 @@ module S       = FStarC.Syntax.Syntax
 module SS      = FStarC.Syntax.Subst
 module U       = FStarC.Syntax.Util
 
-let as_primitive_step is_strong (l, arity, u_arity, f, f_nbe) =
-  FStarC.TypeChecker.Primops.Base.as_primitive_step_nbecbs is_strong (l, arity, u_arity, f, (fun cb univs args -> f_nbe univs args))
+let as_primitive_step is_strong (l, arity, u_arity, (f:interp_t), (f_nbe : nbe_interp_t)) =
+  FStarC.TypeChecker.Primops.Base.as_primitive_step_nbecbs is_strong (l, arity, u_arity, f, f_nbe)
 
-let arg_as_int (a:arg) : option int = fst a |> try_unembed_simple
+let arg_as_int (a:arg) : ML (option int) = fst a |> try_unembed_simple
 
 let arg_as_list {|e:EMB.embedding 'a|} (a:arg)
-: option (list 'a)
+: ML (option (list 'a))
   = fst a |> try_unembed_simple
 
 let mixed_binary_op
-  (as_a : arg -> option 'a)
-  (as_b : arg -> option 'b)
-  (embed_c : Range.t -> 'c -> term)
-  (f : Range.t -> universes -> 'a -> 'b -> option 'c)
+  (as_a : arg -> ML (option 'a))
+  (as_b : arg -> ML (option 'b))
+  (embed_c : Range.t -> 'c -> ML term)
+  (f : Range.t -> universes -> 'a -> 'b -> ML (option 'c))
   (psc : psc)
   (norm_cb : EMB.norm_cb)
   (univs : universes)
   (args : args)
-  : option term
+  : ML (option term)
   = match args with
     | [a;b] ->
        begin
@@ -50,16 +49,16 @@ let mixed_binary_op
     | _ -> None
 
 let mixed_ternary_op
-  (as_a : arg -> option 'a)
-  (as_b : arg -> option 'b)
-  (as_c : arg -> option 'c)
-  (embed_d : Range.t -> 'd -> term)
-  (f : Range.t -> universes -> 'a -> 'b -> 'c -> option 'd)
+  (as_a : arg -> ML (option 'a))
+  (as_b : arg -> ML (option 'b))
+  (as_c : arg -> ML (option 'c))
+  (embed_d : Range.t -> 'd -> ML term)
+  (f : Range.t -> universes -> 'a -> 'b -> 'c -> ML (option 'd))
   (psc : psc)
   (norm_cb : EMB.norm_cb)
   (univs : universes)
   (args : args)
-  : option term
+  : ML (option term)
   = match args with
     | [a;b;c] ->
        begin
@@ -87,29 +86,8 @@ let ops : list primitive_step =
         [S.iarg t; S.as_arg l]
         r
     in
-    (  PC.immutable_array_of_list_lid, 2, 1,
-       mixed_binary_op
-          (fun (elt_t, _) -> Some elt_t) //the first arg of of_list is the element type
-          (fun (l, q) -> //2nd arg: try_unembed_simple as a list term
-            match arg_as_list #_ #FStarC.Syntax.Embeddings.e_any (l, q) with
-            | Some lst -> Some (l, lst)
-            | _ -> None)
-          (fun r (universes, elt_t, (l, blob)) ->
-            //embed the result back as a Tm_lazy with the `ImmutableArray.t term` as the blob
-            //The kind records the type of the blob as IA.t "any"
-            //and the interesting thing here is that the thunk represents the blob back as pure F* term
-            //IA.of_list u#universes elt_t l.
-            //This unreduced representation can be used in a context where the blob doesn't make sense,
-            //e.g., in the SMT encoding, we represent the blob computed by of_list l
-            //just as the unreduced term `of_list l`
-            S.mk (Tm_lazy { blob;
-                            lkind=Lazy_embedding (emb_typ EMB.(emb_typ_of _ #e_any ()), Thunk.mk (fun _ -> un_lazy universes elt_t l r));
-                            ltyp=S.mk_Tm_app (S.mk_Tm_uinst (U.fvar_const PC.immutable_array_t_lid) universes) [S.as_arg elt_t] r;
-                            rng=r }) r)
-          (fun r universes elt_t (l, lst) ->
-            //The actual primitive step computing the IA.t blob
-             let blob = FStar.ImmutableArray.Base.of_list #term lst in
-             Some (universes, elt_t, (l, FStarC.Dyn.mkdyn blob))),
+    let nbe_of_list : nbe_interp_t =
+      fun _cbs univs args ->
        NBETerm.mixed_binary_op
          (fun (elt_t, _) -> Some elt_t)
          (fun (l, q) ->
@@ -117,8 +95,6 @@ let ops : list primitive_step =
            | None -> None
            | Some lst -> Some (l, lst))
          (fun (universes, elt_t, (l, blob)) ->
-           //The embedding is similar to the non-NBE case
-           //But, this time the thunk is the NBE.t representation of `of_list l`
            NBETerm.mk_t <|
            NBETerm.Lazy (Inr (blob, emb_typ EMB.(emb_typ_of _ #e_any ())),
                          Thunk.mk (fun _ ->
@@ -127,10 +103,28 @@ let ops : list primitive_step =
                                                       [NBETerm.as_arg l]))))
          (fun  universes elt_t (l, lst) ->
             let blob = FStar.ImmutableArray.Base.of_list #NBETerm.t lst in
-            Some (universes, elt_t, (l, FStarC.Dyn.mkdyn blob))))
+            Some (universes, elt_t, (l, FStarC.Dyn.mkdyn blob)))
+         univs args
+    in
+    (  PC.immutable_array_of_list_lid, 2, 1,
+       mixed_binary_op
+          (fun (elt_t, _) -> Some elt_t) //the first arg of of_list is the element type
+          (fun (l, q) -> //2nd arg: try_unembed_simple as a list term
+            match arg_as_list #_ #FStarC.Syntax.Embeddings.e_any (l, q) with
+            | Some lst -> Some (l, lst)
+            | _ -> None)
+          (fun r (universes, elt_t, (l, blob)) ->
+            S.mk (Tm_lazy { blob;
+                            lkind=Lazy_embedding (emb_typ EMB.(emb_typ_of _ #e_any ()), Thunk.mk (fun _ -> un_lazy universes elt_t l r));
+                            ltyp=S.mk_Tm_app (S.mk_Tm_uinst (U.fvar_const PC.immutable_array_t_lid) universes) [S.as_arg elt_t] r;
+                            rng=r }) r)
+          (fun r universes elt_t (l, lst) ->
+             let blob = FStar.ImmutableArray.Base.of_list #term lst in
+             Some (universes, elt_t, (l, FStarC.Dyn.mkdyn blob))),
+       nbe_of_list)
   in
   let arg1_as_elt_t (x:arg) : option term = Some (fst x) in
-  let arg2_as_blob (x:arg) : option FStarC.Dyn.dyn =
+  let arg2_as_blob (x:arg) : ML (option FStarC.Dyn.dyn) =
       //try_unembed_simple an arg as a IA.t blob if the emb_typ
       //of the lkind tells us it has the right type
       match (SS.compress (fst x)).n with
@@ -148,35 +142,46 @@ let ops : list primitive_step =
       | _ -> None
   in
   let length_op =
-    let embed_int (r:Range.t) (i:int) : term = embed_simple r i in
-    let run_op (blob:FStarC.Dyn.dyn) : option int =
+    let embed_int (r:Range.t) (i:int) : ML term = embed_simple r i in
+    let run_op (blob:FStarC.Dyn.dyn) : ML (option int) =
         Some (BU.array_length #term (FStarC.Dyn.undyn blob))
+    in
+    let nbe_length : nbe_interp_t =
+      fun _cbs univs args ->
+        NBETerm.mixed_binary_op
+           (fun (elt_t, _) -> Some elt_t)
+           arg2_as_blob_nbe
+           (fun (i:int) -> NBETerm.embed NBETerm.e_int bogus_cbs i)
+           (fun _universes _ blob -> run_op blob)
+           univs args
     in
     ( PC.immutable_array_length_lid, 2, 1,
       mixed_binary_op arg1_as_elt_t //1st arg of length is the type
                       arg2_as_blob //2nd arg is the IA.t term blob
                       embed_int //the result is just an int, so embed it back
                       (fun _r _universes _ blob -> run_op blob),
-      //NBE case is similar
-      NBETerm.mixed_binary_op
-         (fun (elt_t, _) -> Some elt_t)
-         arg2_as_blob_nbe
-         (fun (i:int) -> NBETerm.embed NBETerm.e_int bogus_cbs i)
-         (fun _universes _ blob -> run_op blob) )
+      nbe_length )
   in
   let index_op =
-      (PC.immutable_array_index_lid, 3, 1,
+    let nbe_index : nbe_interp_t =
+      fun _cbs univs args ->
+        NBETerm.mixed_ternary_op
+           (fun (elt_t, _) -> Some elt_t)
+           arg2_as_blob_nbe //2nd arg is an `IA.t NBEterm.t` blob
+           NBETerm.arg_as_int
+           (fun tm -> tm) //In this case, the result is a NBE.t, so embedding is the identity
+           (fun _universes _t blob i  -> Some (BU.array_index #NBETerm.t (FStarC.Dyn.undyn blob) i))
+           univs args
+    in
+    (PC.immutable_array_index_lid, 3, 1,
        mixed_ternary_op arg1_as_elt_t //1st arg of index is the type
                         arg2_as_blob //2nd arg is the `IA.t term` blob
                         arg_as_int //3rd arg is an int
                         (fun r tm -> tm) //the result is just a term, so the embedding is the identity
                         (fun r _universes _t blob i -> Some (BU.array_index #term (FStarC.Dyn.undyn blob) i)),
-      NBETerm.mixed_ternary_op
-         (fun (elt_t, _) -> Some elt_t)
-         arg2_as_blob_nbe //2nd arg is an `IA.t NBEterm.t` blob
-         NBETerm.arg_as_int
-         (fun tm -> tm) //In this case, the result is a NBE.t, so embedding is the identity
-         (fun _universes _t blob i  -> Some (BU.array_index #NBETerm.t (FStarC.Dyn.undyn blob) i)))
+       nbe_index)
   in
-  List.map (as_primitive_step true)
-  [of_list_op; length_op; index_op]
+  let s1 = as_primitive_step true of_list_op in
+  let s2 = as_primitive_step true length_op in
+  let s3 = as_primitive_step true index_op in
+  [s1; s2; s3]
